lib/steel/pulse/Pulse.Typing.Metatheory.Base.fst
@@ -215,7 +215,8 @@ let rec st_typing_weakening g g' t c d g1
     let d_bc = bind_comp_weakening g g' d_bc g1 in
     T_Bind _ e1 e2 c1 c2 b x c d_e1 (magic ()) d_e2 d_bc
 
-  | T_TotBind _ e1 e2 t1 c2 b x _ d_e2 ->
+  | T_TotBind _ e1 e2 t1 u_t1 c2 b x hyp _ _ d_e2 _ ->
+    admit ();
     assume (~ (x `Set.mem` dom g'));
     assume (~ (x `Set.mem` dom g1));
     let d_e2
@@ -239,9 +240,10 @@ let rec st_typing_weakening g g' t c d g1
                   (open_st_term_nv e2 (v_as_nv x))
                   c2 = d_e2 in
     
-    T_TotBind _ e1 e2 t1 c2 b x (magic ()) d_e2
+    T_TotBind _ e1 e2 t1 u_t1 c2 b x hyp (magic ()) (magic ()) d_e2 ()
 
-  | T_GhostBind _ e1 e2 t1 c2 b x _ d_e2 _ ->
+  | T_GhostBind _ e1 e2 t1 u_t1 c2 b x hyp _ _ d_e2 _ _ ->
+    admit ();
     assume (~ (x `Set.mem` dom g'));
     assume (~ (x `Set.mem` dom g1));
     let d_e2
@@ -265,7 +267,7 @@ let rec st_typing_weakening g g' t c d g1
                   (open_st_term_nv e2 (v_as_nv x))
                   c2 = d_e2 in
     
-    T_GhostBind _ e1 e2 t1 c2 b x (magic ()) d_e2 (magic ())
+    T_GhostBind _ e1 e2 t1 u_t1 c2 b x hyp (magic ()) (magic ()) d_e2 () (magic ())
 
 
   | T_If _ b e1 e2 c uc hyp _ d_e1 d_e2 _ ->
@@ -602,26 +604,34 @@ let rec st_typing_subst g x t g' #e #eff e_typing #e1 #c1 e1_typing _
              (coerce_eq (st_typing_subst g x t (push_binding g' y ppname_default (comp_res c1)) e_typing d_e2 (magic ())) ())
              (bind_comp_subst g x t g' e_typing d_bc)
 
-  | T_TotBind _ e1 e2 t1 c2 b y _ d_e2 ->
+  | T_TotBind _ e1 e2 t1 u_t1 c2 b y hyp _ _ d_e2 _ ->
     T_TotBind _ (subst_term e1 ss)
                 (subst_st_term e2 ss)
                 (subst_term t1 ss)
+                u_t1
                 (subst_comp c2 ss)
                 b
                 y
+                hyp
+                (magic ())
                 (magic ())
                 (coerce_eq (st_typing_subst g x t (push_binding g' y ppname_default t1) e_typing d_e2 (magic ())) ())
+                ()
 
-  | T_GhostBind _ e1 e2 t1 c2 b y _ d_e2 _ ->
+  | T_GhostBind _ e1 e2 t1 u_t1 c2 b y hyp _ _ d_e2 _ _ ->
     T_GhostBind _ (subst_term e1 ss)
-                (subst_st_term e2 ss)
-                (subst_term t1 ss)
-                (subst_comp c2 ss)
-                b
-                y
-                (magic ())
-                (coerce_eq (st_typing_subst g x t (push_binding g' y ppname_default t1) e_typing d_e2 (magic ())) ())
-                (magic ())
+                  (subst_st_term e2 ss)
+                  (subst_term t1 ss)
+                  u_t1
+                  (subst_comp c2 ss)
+                  b
+                  y
+                  hyp
+                  (magic ())
+                  (magic ())
+                  (coerce_eq (st_typing_subst g x t (push_binding g' y ppname_default t1) e_typing d_e2 (magic ())) ())
+                  ()
+                  (magic ())
 
   | T_If _ b e1 e2 c uc hyp _ d_e1 d_e2 _ ->
     T_If _ (subst_term b ss)
